

# Lambda Calculus II

4190.310  
Programming Languages  
Spring 2014

Lecture 03

Reading assignments: Chapter 10

# Call-by-value

- Given an application  $(\lambda x.t) s$ ,  $s$  is a value before calling the function
  - Reduce leftmost-outermost redex where argument is a value
  - Given an application  $st$ , we first evaluate  $s$  until it is a value then we evaluate  $t$  until it is a value
    - Then, apply the function to the value
- Value
  - $\lambda$ -abstraction (pure lambda calculus)
  - An expression that cannot be reduced/simplified any further

$$\begin{aligned} & (\lambda x.\lambda y.y\ x)(5+4)(\lambda x.x + 1) \\ &= (\lambda x.\lambda y.y\ x)\ 9\ (\lambda x.x + 1) \\ &= (\lambda y.y\ 9)\ (\lambda x.x + 1) \\ &= (\lambda x.x + 1)\ 9 \\ &= 9 + 1 \\ &= 10 \end{aligned}$$

# Call-by-name

- Apply the function as soon as possible
  - Reduce the leftmost-outermost redex, but not inside abstractions

$$\begin{aligned} & (\lambda x. \lambda y. y \ x)(5+4)(\lambda x. x + 1) \\ &= (\lambda y. y \ (5+4))(\lambda x. x + 1) \\ &= (\lambda x. x + 1) \ (5+4) \\ &= (5+4) + 1 \\ &= 9 + 1 \\ &= 10 \end{aligned}$$

# Call-by-value vs. Call-by-name

- When answers are the same, the order of evaluation may be different

$$\begin{aligned} & (\lambda x.x \ 6)((\lambda y.y \ y)(\lambda x.x)) \\ &= (\lambda x.x \ 6)((\lambda x.x) \ (\lambda x.x)) \\ &= (\lambda x.x \ 6)(\lambda x.x) \\ &= (\lambda x.x) \ 6 \\ &= 6 \end{aligned}$$

$$\begin{aligned} & (\lambda x.x \ 6)((\lambda y.y \ y)(\lambda x.x)) \\ &= ((\lambda y.y \ y)(\lambda x.x)) \ 6 \\ &= ((\lambda x.x)(\lambda x.x)) \ 6 \\ &= (\lambda x.x) \ 6 \\ &= 6 \end{aligned}$$

# $\eta$ -equivalence

- Two functions are the same iff they give the same result for all arguments
- $\lambda x.Mx = M$ , where  $x$  is not free in  $M$

# Polymorphic Functions

- $\lambda x.x$
- Identity function
  - $(\lambda x.x) M = M$  for any lambda expression  $M$
- Functions that allow arguments of many types are known as polymorphic functions
  - $\lambda x.x$  acts as an identity function on the set of integers, on a set of functions of some type, or on any other kind of object

# Functions of Several Arguments

- Functions with two arguments  $x$  and  $y$  may be represented by
  - $\lambda x.(\lambda y.M)$
- $f(g, x) = g(x)$
- $f_{\text{curry}} = \lambda g.(\lambda x. g\ x)$ 
  - Invented by Schönfinkel, but named after Haskell Curry

# Numbers

- Numbers are defined as functions
  - The number of times a function parameter is applied
  - $0 = \lambda s. \lambda z. z$
  - $1 = \lambda s. \lambda z. s z$
  - $2 = \lambda s. \lambda z. s(s z)$
  - $3 = \lambda s. \lambda z. s(s(s z))$
  - ...



# Successor Function

- Successor function
  - $S = \lambda w. \lambda y. \lambda x. y(wyx)$

$$\begin{aligned} S(o) &= (\lambda w. \lambda y. \lambda x. y(wyx))o \\ &= (\lambda w. \lambda y. \lambda x. y(wyx))(\lambda s. \lambda z. z) \\ &= \lambda y. \lambda x. y((\lambda s. \lambda z. z)yx) \\ &= \lambda y. \lambda x. y((\lambda z. z)x) \\ &= \lambda y. \lambda x. yx \\ &= \lambda s. \lambda z. sz \end{aligned}$$

# Addition

- $M + N = M \ S \ N$ 
  - Apply the successor function  $M$  times to  $N$
- $2 + 3$

$$\begin{aligned} 2S3 &= (\lambda s.\lambda z.s(sz))(\lambda w.\lambda y.\lambda x.y(wyx))3 \\ &= (\lambda z.(\lambda w.\lambda y.\lambda x.y(wyx))((\lambda w.\lambda y.\lambda x.y(wyx)) z)3) \\ &= (\lambda w.\lambda y.\lambda x.y(wyx))((\lambda w.\lambda y.\lambda x.y(wyx)) 3) \\ &= S(S3) \\ &= S4 \\ &= 5 \end{aligned}$$

# Multiplication

- $M = \lambda xyz.x(yz)$

$$\begin{aligned}
 M22 &= (\lambda xyz.x(yz))\ 2\ 2 \\
 &= \lambda yz.2(yz)\ 2 \\
 &= \lambda z.2(2\ z) \\
 &= \lambda z.2((\lambda v.\lambda w.v(vw))\ z) \\
 &= \lambda z.2(\lambda w.z(zw)) \\
 &= \lambda z.(\lambda v.\lambda w.v(vw))N \\
 &\quad (\text{let } N = (\lambda w.z(zw))) \\
 &= \lambda z.(\lambda w.N(Nw)) \\
 &= \lambda z.(\lambda w.N((\lambda w.z(zw))\ w)) \\
 &= \lambda z.(\lambda w.N(z(zw))) \\
 &= \lambda z.(\lambda w.(\lambda w.z(zw))(z(zw))) \\
 &= \lambda z.(\lambda w.(\lambda x.z(zx))(z(zw))) \\
 &= \lambda z.(\lambda w.(z(z(z(zw)))))) \\
 &= 4
 \end{aligned}$$

# Conditionals and Logical Operations

- $T = \lambda xy.x$
- $F = \lambda xy.y$ 
  - $Fz = \lambda y.y$  (identity function)
- $\wedge = \lambda xy.xyF$
- $\vee = \lambda xy.xTy$
- $\sim = \lambda x.xFT$

$$\begin{aligned}\sim T &= (\lambda x.xFT)T \\ &= TFT \\ &= (\lambda xy.x)FT \\ &= F\end{aligned}$$

# A Conditional Test

- A function that is true if a number is 0 and false otherwise
- $Z = \lambda x.xF \sim F \lambda s.\lambda z.z$

$$\begin{aligned}
 Z0 &= (\lambda x.xF \sim F)0 \\
 &= (\lambda s.\lambda z.z)F \sim F \\
 &= (\lambda z.z) \sim F \\
 &= (\lambda z.z)((\lambda x.xFT))F \\
 &= (\lambda x.xFT)F \\
 &= FFT \\
 &= T
 \end{aligned}$$

$$\begin{aligned}
 Z3 &= (\lambda x.xF \sim F)3 \\
 &= 3F \sim F \\
 &= (\lambda s.\lambda z.s(s(s(z))))F \sim F \\
 &= F(F(F \sim))F \\
 &= IF \quad (I = \lambda x.x) \\
 &= F
 \end{aligned}$$

# Predecessor Function

- A pair (a, b) can be represented using the following function
  - $\text{PAIR} = \lambda a. \lambda b. \lambda x. xab$
  - $\text{FIRST} = \lambda p. pT$
  - $\text{SECOND} = \lambda p. pF$

# Predecessor Function

- The following function generates the pair  $(n+1, n)$  from the pair  $(n, m)$ 
  - $\Phi = \lambda p. \text{PAIR} (\text{S}(\text{FIRST } P)) (\text{FIRST } p)$
  - A new pair is formed using  $pT$ , then it is incremented in the first position and just copied for the second position
- The predecessor of a number  $n$  is obtained by applying  $n$  times the function  $\Phi$  to the pair  $(0, 0)$  and then selecting the second member of the new pair
  - $P = \lambda n. \text{SECOND}(n \Phi (\text{PAIR } 0 \ 0))$
  - $P(P_1) = P_0 = \text{SECOND}(0 \Phi (\text{PAIR } 0 \ 0)) = 0$

# Equality

- A function that tests if a number  $x$  is greater than or equal to a number  $y$ 
  - $GE = \lambda x. \lambda y. Z(xPy)$
- Equality test
  - If  $x \geq y$  and  $x \leq y$ , then  $x = y$
  - $EQ = \lambda x. \lambda y. \wedge (Z(xPy)) (Z(xPy))$

$$\begin{aligned}
 GE\ 3\ 4 &= (\lambda x. \lambda y. Z(xPy))\ 3\ 4 \\
 &= Z(3P4) \\
 &= Z\ 1 \\
 &= F
 \end{aligned}$$

$$\begin{aligned}
 GE\ 4\ 2 &= (\lambda x. \lambda y. Z(xPy))\ 4\ 2 \\
 &= Z(4P2) \\
 &= Z\ 0 \\
 &= T
 \end{aligned}$$

$$\begin{aligned}
 EQ\ 2\ 2 &= (\lambda x. \lambda y. \wedge (Z(xPy)) (Z(xPy)))\ 2\ 2 \\
 &= \wedge (Z(2P2)) (Z(2P2)) \\
 &= \wedge\ T\ T \\
 &= T
 \end{aligned}$$



# Recursion

- A fixed point of a function  $G$  is a value  $f$  such that  $f = G(f)$
- A function that calls a function  $y$  and then regenerates itself
  - Fixed-point operator
  - $Y = \lambda y.(\lambda x.y(xx))(\lambda x.y(xx))$
  - $Yf$  is a fixed point of  $f$

$$\begin{aligned} Yf &= (\lambda y.(\lambda x.y(xx))(\lambda x.y(xx))) f \\ &= (\lambda x.f(xx))(\lambda x.f(xx)) \\ &= f((\lambda x.f(xx))(\lambda x.f(xx))) \\ &= f(Yf) \end{aligned}$$

# Recursive Summation

- A function that adds up the first  $n$  natural numbers
  - $f(0) = 0$
  - $f(n) = n + f(n-1)$
  - If  $n$  is 0 the result is 0
  - Otherwise, the successor function is applied  $n$  times to the recursive call of the function applied to the predecessor of  $n$
- $f = \lambda r. \lambda n. Z\ n\ 0\ (n\ S\ (r(Pn)))$

# Recursive Summation

$$\begin{aligned}
 Y\ f\ 3 &= (\lambda y.(\lambda x.y(xx))(\lambda x.y(xx)))\ f\ 3 \\
 &= f\ (Yf)\ 3 \\
 &= (\lambda r.\lambda n. Z\ n\ o\ (n\ S\ (r(Pn))))\ (Yf)\ 3 \\
 &= (\lambda n. Z\ n\ o\ (n\ S\ ((Yf)(Pn))))\ 3 \\
 &= Z\ 3\ o\ (3\ S\ ((Yf)(P\ 3))) \\
 &= F\ o\ (3\ S\ ((Yf)(P\ 3))) \\
 &= 3\ S\ ((Yf)(P\ 3)) \\
 &= 3\ S\ ((Yf)\ 2) \\
 &= 3\ S\ (2\ S\ ((Yf)\ 1)) \\
 &= 3\ S\ (2\ S\ (1\ S\ ((Yf)\ o))) \\
 &= 3\ S\ (2\ S\ (1\ S\ (Z\ o\ o\ (o\ S\ ((Yf)(P\ o)))))) \\
 &= 3\ S\ (2\ S\ (1\ S\ o)) \\
 &= 6
 \end{aligned}$$